reduce/PingMany.v
@@ -1,0 +1,22 @@
+Require Export ProcessRewrite.
+Require Export RewriteTactics.
+
+Inductive PingPong :=
+| Ping : PingPong
+| Pong : PingPong.
+
+Example PingPong_many :
+  forall (q x : nat) (ps : SetVar),
+    q <> x ->
+    [ { ps } [[ s_send (p_sng q) (Ping, p_set ps); x ~ (s_recv (Pong, p_sng x)) ]]
+    |   q  [[ s_iter ps
+              (x ~ (s_recv (Ping, p_sng x); s_send (p_sng x) (Pong, p_sng q)))]] ]
+    ===> [ { ps } [[ s_skip ]] | q [[ s_skip ]] ].
+Proof.
+  intros.
+  inst_bind 1.
+  reduce_pair 0 1.
+  inst_bind 0.
+  reduce_pair 0 1.
+  skip.
+Qed.
