reduce/ProcessRewrite.v
@@ -1,0 +1,265 @@
+Require Export List.
+Import ListNotations.
+Require Export Setoid.
+Require Export Morphisms.
+Require Export SetoidTactics.
+Require Import RelationClasses.
+Require Export Coq.Structures.Orders.
+
+Set Implicit Arguments.
+Unset Strict Implicit.
+
+Section Process.
+  Context {T : Type}.
+  Context {eq_dec_T : forall (t1 t2 : T), {t1 = t2}+{t1 <> t2}}.
+  Definition pid := nat.
+  Inductive SetVar :=
+    | X : nat -> SetVar.
+  Inductive MuVar :=
+    | L : nat -> MuVar.
+  Definition eq_dec_pid := PeanoNat.Nat.eq_dec. 
+
+  Inductive PidClass : Type :=
+  | p_none : PidClass
+  | p_sng  : pid -> PidClass
+  | p_set  : SetVar -> PidClass.
+  
+  Definition eqb_setvar (xs ys : SetVar) : bool :=
+    match (xs, ys) with
+      | (X xs, X ys) => Nat.eqb xs ys
+    end.
+  
+  Definition eqb_pidclass (p q : PidClass) :=
+    match p, q with
+      | p_none, p_none => true
+      | p_sng p', p_sng q' => Nat.eqb p' q'
+      | p_set ps, p_set qs => eqb_setvar ps qs
+      | _,_ => false
+    end.
+        
+  Definition eq_dec_pidclass : forall (p q : PidClass), {p=q}+{p<>q}.
+  Proof. repeat decide equality. Qed.
+  
+  Lemma eqb_pidclass_eq : 
+    forall (p q : PidClass),
+      eqb_pidclass p q = true <-> p = q.
+  Proof.
+    intros.
+    destruct (eq_dec_pidclass p q). subst.
+    split; intros. reflexivity. 
+    destruct q. reflexivity. simpl. induction p; auto.
+    simpl. destruct s. unfold eqb_setvar. induction n; auto.
+    destruct p; destruct q; split; intros; try inversion H; try congruence.
+    apply PeanoNat.Nat.eqb_eq in H1. subst. reflexivity.
+    destruct s; destruct s0.
+    apply PeanoNat.Nat.eqb_eq in H1. subst. reflexivity.
+  Qed. 
+
+  Definition M := (T * PidClass)%type.
+
+  Definition subst_pid_m (p1 : PidClass) (p2 : PidClass) (m : M) :=
+    match (p1, m) with
+      | (p_sng pid1, (t, p_sng pid2)) => 
+        if eq_dec_pid pid1 pid2 then
+          (t, p2)
+          else m
+      | _ =>  m
+    end.
+    
+  Inductive Stmt : Type :=
+  | s_skip  : Stmt
+  | s_bind  : PidClass -> Stmt -> Stmt
+  | s_send  : PidClass -> M -> Stmt
+  | s_recv  : M -> Stmt
+  | s_seq   : Stmt -> Stmt -> Stmt
+  | s_iter  : SetVar -> Stmt -> Stmt
+  | s_loop  : MuVar -> Stmt -> Stmt
+  | s_var   : MuVar -> Stmt
+  (* These statements below never appear in original programs *)
+  | s_loop_body : MuVar -> Stmt -> Stmt
+  | s_loop_end  : MuVar -> Stmt -> Stmt.
+
+  
+  Definition Process := (PidClass * Stmt)%type.
+  Definition Config := list Process.
+  
+  Definition nth_config (c : Config) (n : nat) := nth_error c n.
+  Fixpoint update_nth (c : Config) (n : nat) (ps : PidClass * Stmt) := 
+    match (n, c) with
+      | (O, _::cs) => ps::cs
+      | (_, [])    => c
+      | (S n, ps'::cs') => ps' :: update_nth cs' n ps
+    end.
+  
+  Inductive EqStmt : Stmt -> Stmt -> Prop :=
+    | stmt_refl : forall (s : Stmt), EqStmt s s 
+    | stmt_sym : forall (s t : Stmt), 
+      EqStmt s t -> EqStmt t s
+    | stmt_trans : forall (s t u : Stmt), 
+      EqStmt s t -> EqStmt t u -> EqStmt s u
+    | stmt_skip1 : forall (s : Stmt),
+      EqStmt s (s_seq s s_skip)
+    | stmt_skip2 : forall (s : Stmt),
+      EqStmt s (s_seq s_skip s).
+  
+  Instance EqStmt_equiv : Equivalence EqStmt := _.
+  Proof.
+    refine (Build_Equivalence _ _ _ _); hnf; intros.
+    apply stmt_refl.
+    eauto using stmt_sym.
+    eauto using stmt_trans.
+  Defined.
+   
+  Inductive Context :=
+  | Mult : SetVar -> Context
+  | Loop : MuVar -> Context.
+
+  Fixpoint head_stmt' s stk :=
+    match s with
+      | s_seq s' _       => head_stmt' s' stk
+      | s_iter xs s'     => head_stmt' s' (Mult xs :: stk)
+      | s_loop_body x s' => head_stmt' s' (Loop x  :: stk)
+      | s_loop_end x s'  => head_stmt' s' stk
+      | s'               => (s',stk)
+    end.
+
+  Definition head_stmt s := head_stmt' s [].
+  
+  Fixpoint rest_stmt s :=
+    match s with
+      | s_seq s' t  => match rest_stmt s' with
+                         | s_skip => t
+                         | s''    => s_seq s'' t
+                       end
+      | s_iter xs t => match rest_stmt t with
+                         | s_skip => s_skip
+                         | t'     => s_iter xs t'
+                       end
+      | s_loop_body x t => s_loop_body x (rest_stmt t)
+      (* | s_loop x t  => s_loop x (rest_stmt t) *)
+      | _           => s_skip
+    end.
+  
+  Definition get_pid  (x : PidClass * (Stmt * list Context)) := fst x.
+  Definition get_stmt (x : PidClass * (Stmt * list Context)) := fst (snd x).
+  Definition get_ctx  (x : PidClass * (Stmt * list Context)) := snd (snd x).
+  
+  Definition eq_dec_m : forall m1 m2 : M, {m1=m2}+{m1<>m2}.
+  Proof. repeat decide equality. Qed.
+  
+  Definition elim ps qs :=
+    match (get_stmt ps, get_stmt qs) with
+      | (s_send q m, s_recv m') => 
+        if (eq_dec_m m m') then eqb_pidclass q (get_pid qs) else false
+      | (s_recv m', s_send p m) => 
+        if (eq_dec_m m m') then eqb_pidclass p (get_pid ps) else false
+      | _ => false
+    end.
+  
+  Definition Elim ps qt :=
+    match (get_stmt ps, get_stmt qt) with
+      | (s_send q m, s_recv m') => 
+        q = get_pid qt /\ m = m'
+      | (s_recv m, s_send p m') => p = get_pid ps /\ m = m'
+      | _ => False
+    end.
+  
+  Lemma elim_Elim :
+    forall ps qs : PidClass * (Stmt * list Context),
+      elim ps qs = true -> Elim ps qs.
+  Proof.
+    intros.
+    destruct ps as [p [ps pc]]; destruct qs as [q [qs qc]]. 
+    induction ps; destruct qs; try inversion H.
+    unfold elim in H1.
+    unfold get_stmt in H1.
+    simpl in H1.
+    destruct (eq_dec_m m m0). apply eqb_pidclass_eq in H1. subst.  
+    cbv. auto. congruence.
+    unfold elim in H. unfold get_stmt in H. simpl in H.
+    destruct (eq_dec_m m0 m). apply eqb_pidclass_eq in H. subst.
+    cbv. auto. congruence.
+  Qed.
+    
+  Definition MatchCtxt ps qt :=
+    match (get_pid ps, get_pid qt, get_ctx ps, get_ctx qt) with
+      | (p_sng p', p_sng q', c1, c2) => c1 = c2
+      | (p_set ps, p_sng q', [], [Mult ps']) => ps = ps'
+      | (p_sng p', p_set qs, [Mult qs'], []) => qs = qs'
+      | _ => False
+    end.
+  
+  Definition subst_pid p q p' :=
+    match (p, p') with
+      | (p_sng p, p_sng pid') => if eq_dec_pid p pid' then q else p'
+      | _ => p'
+    end.
+  
+  Fixpoint subst_stmt p q s :=
+    match s with
+      | s_skip => s_skip
+      | s_send p' m => s_send (subst_pid p q p') (subst_pid_m p q m)
+      | s_recv m => s_recv (subst_pid_m p q m)
+      | s_seq s' t' => s_seq (subst_stmt p q s') (subst_stmt p q t')
+      | _ => s
+    end.
+  
+  Fixpoint inst_stmt (p q : PidClass) s :=
+    match s with
+      | s_seq t u => s_seq (inst_stmt p q t) (inst_stmt p q u)
+      | s_iter xs s => s_iter xs (inst_stmt p q s)
+      | s_loop x s => s_loop x (inst_stmt p q s)
+      | s_bind x s => 
+        match (x, p) with
+          | (p_sng x', p_sng p') => 
+            if eq_dec_pid x' p' then subst_stmt p q s else s
+          | _ => s
+        end
+      | _ => s
+    end.
+        
+  Inductive RewriteRel : Config -> Config -> Prop :=
+  | rewrite_refl : forall (c : Config), RewriteRel c c
+
+  | rewrite_trans :
+    forall (c1 c2 c3 : Config),
+      RewriteRel c1 c2 -> RewriteRel c2 c3 ->
+      RewriteRel c1 c3
+
+  | rewrite_bind :
+    forall (c : Config) (i : nat) (p x q : PidClass) (s t : Stmt),
+      nth_config c i = Some (p, s) ->
+      fst (head_stmt s) = s_bind x t ->
+      RewriteRel c (update_nth c i (p, inst_stmt x q s))
+                 
+  | rewrite_unroll_loop :
+    forall (c : Config) (i : nat) (p : PidClass) (s t : Stmt) (X : MuVar),
+      nth_config c i = Some (p, s) ->
+      fst (head_stmt s) = s_loop X t ->
+      RewriteRel c (update_nth c i (p, s_seq (s_loop_body X t) (s_loop X s)))
+                 
+  | rewrite_elim_unroll :
+    forall (c : Config) (i : nat) (p : PidClass) (s : Stmt) (X : MuVar),
+      nth_config c i = Some (p, s) ->
+      fst (head_stmt s) = s_var X ->
+      hd_error (snd (head_stmt s)) = Some (Loop X) ->
+      RewriteRel c (update_nth c i (p, rest_stmt s))
+
+  | rewrite_pair :
+    forall (c : Config) (i1 i2 : nat) (p1 p2 : PidClass) (s1 s2 : Stmt),
+      nth_config c i1 = Some (p1, s1) -> 
+      nth_config c i2 = Some (p2, s2) ->
+      Elim (p1, head_stmt s1) (p2, head_stmt s2) ->
+      MatchCtxt (p1, head_stmt s1) (p2, head_stmt s2) ->
+      RewriteRel c (update_nth (update_nth c i1 (p1, rest_stmt s1)) i2 (p2, rest_stmt s2)).
+  Hint Constructors RewriteRel : rewrite.
+  
+End Process.
+
+Notation "[ x ]" := (cons x nil).
+Notation "[ x | .. | y ]" := (cons x .. (cons y nil) ..).
+Notation "P1 ; P2" := (s_seq P1 P2) (at level 65, right associativity).
+Notation "P [[ S ]]" := (p_sng P, S) (at level 80).
+Notation "{ P } [[ S ]]" := (p_set P, S) (at level 80).
+Notation "C1 ===> C2" := (RewriteRel C1 C2) (at level 95).
+Notation "X ~ S" := (s_bind (p_sng X) S) (at level 60).
