reduce/RewriteTactics.v
@@ -1,0 +1,24 @@
+Require Export ProcessRewrite.
+
+Ltac skip := solve[apply rewrite_refl].
+
+Ltac apply_rewrite x :=
+  eapply rewrite_trans; [ x | idtac].
+
+Ltac reduce_pair i j :=
+  eapply rewrite_trans;
+    [apply rewrite_pair with (i1 := i) (i2 := j); try reflexivity | idtac]; cbv; auto.
+
+Ltac expand_subst :=
+  simpl; simpl inst_stmt; simpl subst_stmt; unfold subst_pid_m, subst_pid;
+    repeat match goal with
+             | |- context[eq_dec_pid ?x ?x] =>
+               destruct (eq_dec_pid x x); [ idtac | congruence]
+             | |- context[eq_dec_pid ?x ?y] =>
+               destruct (eq_dec_pid x y); [ congruence | idtac]
+           end.
+
+Ltac inst_bind i x :=
+  eapply rewrite_trans; [
+    eapply rewrite_bind with (1 := i) (3 := x); simpl; try reflexivity
+    | expand_subst].
